src/program_proof/rsm/mpaxos_proof.v
@@ -1,0 +1,330 @@
+From Perennial.program_proof Require Import grove_prelude.
+From Perennial.program_logic Require Import atomic. (* prefer the ncfupd atomics *)
+From Goose.github_com.mit_pdos.rsm Require Import mpaxos.
+
+(* TODO: move to mpaxos_ghost.v once stable *)
+Class mpaxos_ghostG (Σ : gFunctors).
+
+Record mpaxos_names := {}.
+
+Section consensus.
+  Context `{!mpaxos_ghostG Σ}.
+  (* TODO: remove this once we have real defintions for resources. *)
+  Implicit Type (γ : mpaxos_names).
+
+  (* Definitions. *)
+  Definition own_consensus γ (l : list string) : iProp Σ.
+  Admitted.
+
+  Definition own_consensus_half γ (l : list string) : iProp Σ.
+  Admitted.
+
+  Definition is_consensus_lb γ (l : list string) : iProp Σ.
+  Admitted.
+
+  Definition own_candidates γ (vs : gset string) : iProp Σ.
+  Admitted.
+
+  Definition own_candidates_half γ (vs : gset string) : iProp Σ.
+  Admitted.
+
+  (* Type class instances. *)
+  #[global]
+  Instance is_consensus_lb_persistent γ l :
+    Persistent (is_consensus_lb γ l).
+  Admitted.
+
+  (* Rules. *)
+  Lemma consensus_update {γ} l1 l2 vs :
+    Forall (λ x, x ∈ vs) l2 ->
+    prefix l1 l2 ->
+    own_consensus γ l1 -∗
+    own_candidates_half γ vs ==∗
+    own_consensus γ l2 ∗ own_candidates_half γ vs.
+  Admitted.
+
+  Lemma consensus_witness {γ l} :
+    own_consensus_half γ l -∗
+    is_consensus_lb γ l.
+  Admitted.
+
+  Lemma consensus_combine {γ l1 l2} :
+    own_consensus_half γ l1 -∗
+    own_consensus_half γ l2 -∗
+    own_consensus γ l1 ∧ ⌜l1 = l2⌝.
+  Admitted.
+
+  Lemma consensus_split {γ l} :
+    own_consensus γ l -∗
+    own_consensus_half γ l ∗ own_consensus_half γ l.
+  Admitted.
+
+  Lemma consensus_prefix {γ l1 l2} :
+    own_consensus_half γ l1 -∗
+    is_consensus_lb γ l2 -∗
+    ⌜prefix l2 l1⌝.
+  Admitted.
+
+  Lemma consensus_lb_prefix {γ l1 l2} :
+    is_consensus_lb γ l1 -∗
+    is_consensus_lb γ l2 -∗
+    ⌜prefix l1 l2 ∨ prefix l2 l1⌝.
+  Admitted.
+
+  Lemma candidates_update {γ vs1} vs2 :
+    vs1 ⊆ vs2 ->
+    own_candidates γ vs1 ==∗
+    own_candidates γ vs2.
+  Admitted.
+
+  Lemma candidates_combine {γ vs1 vs2} :
+    own_candidates_half γ vs1 -∗
+    own_candidates_half γ vs2 -∗
+    own_candidates γ vs1 ∧ ⌜vs1 = vs2⌝.
+  Admitted.
+
+  Lemma candidates_split {γ vs} :
+    own_candidates γ vs -∗
+    own_candidates_half γ vs ∗ own_candidates_half γ vs.
+  Admitted.
+
+  Lemma consensus_incl {γ l vs} :
+    own_consensus_half γ l -∗
+    own_candidates_half γ vs -∗
+    ⌜Forall (λ x, x ∈ vs) l⌝.
+  Admitted.
+End consensus.
+(* TODO: move to mpaxos_ghost.v once stable *)
+
+(* TODO: move to mpaxos_propose/lookup.v once stable *)
+Section prog.
+  Context `{!heapGS Σ, !mpaxos_ghostG Σ}.
+
+  Definition mpaxosN := nroot .@ "mpaxos".
+
+  Definition is_paxos (paxos : loc) (nid : u64) (sc : nat) (γ : mpaxos_names) : iProp Σ.
+  Admitted.
+
+  (* TODO: remove this once is_paxos defined. *)
+  #[global]
+  Instance is_paxos_persistent px nid sc γ :
+    Persistent (is_paxos px nid sc γ).
+  Admitted.
+
+  Theorem wp_Paxos__Propose (px : loc) (v : string) nid sc γ :
+  is_paxos px nid sc γ -∗
+  {{{ True }}}
+  <<< ∀∀ vs, own_candidates_half γ vs >>>
+    Paxos__Propose #px #(LitString v) @ ↑mpaxosN
+  <<< own_candidates_half γ ({[v]} ∪ vs) >>>
+  {{{ (lsn : u64) (term : u64), RET (#lsn, #term); True }}}.
+  Admitted.
+
+  Theorem wp_Paxos__Lookup (px : loc) (i : u64) nid sc γ :
+    is_paxos px nid sc γ -∗
+    {{{ True }}}
+    <<< ∀∀ l, own_consensus_half γ l >>>
+      Paxos__Lookup #px #i @ ↑mpaxosN
+    <<< ∃∃ l', own_consensus_half γ l' >>>
+    {{{ (v : string) (ok : bool), RET (#(LitString v), #ok);
+        ⌜if ok then l' !! (int.nat i) = Some v else True⌝
+    }}}.
+  Admitted.
+
+  Definition paxos_init px γ : iProp Σ :=
+  "Hvs"  ∷ own_candidates_half γ ∅ ∗
+  "Hv"   ∷ own_consensus_half γ [] ∗
+  "#Hpx" ∷ is_paxos px (U64 0) 3%nat γ.
+
+  Theorem wp_MkPaxos :
+    {{{ True }}}
+      MkPaxos #()
+      {{{ (γ : mpaxos_names) (px : loc), RET #px; paxos_init px γ }}}.
+  Proof.
+    (*@ func MkPaxos() *Paxos {                                                 @*)
+    (*@     var px *Paxos                                                       @*)
+    (*@                                                                         @*)
+    (*@     return px                                                           @*)
+    (*@ }                                                                       @*)
+  Admitted.
+
+End prog.
+(* TODO: move to mpaxos_propose/lookup.v once stable *)
+
+(* TODO: move to mpaxos_examples.v once stable *)
+Section prog.
+  Context `{!heapGS Σ, !mpaxos_ghostG Σ}.
+
+  Definition of_length_five s := String.length s = 5%nat.
+
+  Definition length_of_consensus l :=
+    Forall of_length_five l.
+
+  Definition length_of_candidates (vs : gset string) :=
+    set_Forall of_length_five vs.
+
+  Definition inv_example1 γ : iProp Σ :=
+    ∃ l vs,
+      "Hl"  ∷ own_consensus_half γ l ∗
+      "Hvs" ∷ own_candidates_half γ vs ∗
+      "%Hlenl"  ∷ ⌜length_of_consensus l⌝ ∗
+      "%Hlenvs" ∷ ⌜length_of_candidates vs⌝.
+
+  #[global]
+  Instance inv_example1_timeless γ :
+    Timeless (inv_example1 γ).
+  Admitted.
+
+  Definition example1N := nroot .@ "example1N".
+  Definition know_inv_example1 γ : iProp Σ :=
+    inv example1N (inv_example1 γ).
+
+  Lemma prefix_lookup_same_index {A : Type} {l1 l2 : list A} {i v1 v2} :
+    prefix l1 l2 ∨ prefix l2 l1 ->
+    l1 !! i = Some v1 ->
+    l2 !! i = Some v2 ->
+    v1 = v2.
+  Admitted.
+
+  Theorem wp_example1 :
+    {{{ True }}}
+      example1 #()
+    {{{ RET #(); True }}}.
+  Proof using heapGS0 mpaxos_ghostG0 Σ.
+    iIntros (Φ) "_ HΦ".
+    wp_call.
+
+    (*@ func example1() {                                                       @*)
+    (*@     px := MkPaxos()                                                     @*)
+    (*@                                                                         @*)
+    wp_apply wp_MkPaxos.
+    iIntros (γ px) "Hinit".
+    iNamed "Hinit".
+    wp_pures.
+    iMod (inv_alloc example1N _ (inv_example1 γ) with "[Hv Hvs]") as "#Hinvapp".
+    { do 2 iExists _. iFrame. unfold length_of_consensus. set_solver. }
+
+    (*@     i1, _ := px.Propose("hello")                                        @*)
+    (*@                                                                         @*)
+    wp_apply (wp_Paxos__Propose with "Hpx").
+    iInv "Hinvapp" as "> HinvO" "HinvC".
+    iNamed "HinvO".
+    iApply ncfupd_mask_intro; first set_solver.
+    iIntros "Hmask".
+    iExists vs. iFrame.
+    iIntros "Hvs".
+    iMod "Hmask" as "_".
+    iMod ("HinvC" with "[Hl Hvs]") as "_".
+    { do 2 iExists _. iFrame.
+      iPureIntro. split; first done.
+      unfold length_of_candidates.
+      apply set_Forall_union; last done.
+      by rewrite set_Forall_singleton.
+    }
+    iIntros "!>" (lsn term) "_".
+    wp_pures.
+    clear Hlenl Hlenvs l vs.
+
+    (*@     px.Propose("world")                                                 @*)
+    (*@                                                                         @*)
+    wp_apply (wp_Paxos__Propose with "Hpx").
+    iInv "Hinvapp" as "> HinvO" "HinvC".
+    iNamed "HinvO".
+    iApply ncfupd_mask_intro; first set_solver.
+    iIntros "Hmask".
+    iExists vs. iFrame.
+    iIntros "Hvs".
+    iMod "Hmask" as "_".
+    iMod ("HinvC" with "[Hl Hvs]") as "_".
+    { do 2 iExists _. iFrame.
+      iPureIntro. split; first done.
+      unfold length_of_candidates.
+      apply set_Forall_union; last done.
+      by rewrite set_Forall_singleton.
+    }
+    iIntros "!>" (lsn' term') "_".
+    wp_pures.
+    clear Hlenl Hlenvs l vs lsn' term'.
+
+    (*@     // Notice in the proof how we transfer the invariant from the candidate set @*)
+    (*@     // to the consensus.                                                @*)
+    (*@     v1, ok1 := px.Lookup(i1)                                            @*)
+    (*@                                                                         @*)
+    wp_apply (wp_Paxos__Lookup with "Hpx").
+    iInv "Hinvapp" as "> HinvO" "HinvC".
+    iNamed "HinvO".
+    iApply ncfupd_mask_intro; first set_solver.
+    iIntros "Hmask".
+    iExists l. iFrame.
+    iIntros (l1) "Hl1".
+    iDestruct (consensus_witness with "Hl1") as "#Hlb1".
+    iMod "Hmask" as "_".
+    iMod ("HinvC" with "[Hl1 Hvs]") as "_".
+    { iDestruct (consensus_incl with "Hl1 Hvs") as %Hin.
+      do 2 iExists _. iFrame.
+      iPureIntro. split; last done.
+      unfold length_of_consensus.
+      unfold length_of_candidates in Hlenvs.
+      rewrite Forall_forall.
+      intros x Hx.
+      rewrite Forall_forall in Hin.
+      specialize (Hin _ Hx).
+      by specialize (Hlenvs _ Hin).
+    }
+    iIntros "!>" (v1 ok1 Hv1).
+    wp_pures.
+    clear Hlenl Hlenvs l vs.
+
+    (*@     v2, ok2 := px.Lookup(i1)                                            @*)
+    (*@                                                                         @*)
+    wp_apply (wp_Paxos__Lookup with "Hpx").
+    iInv "Hinvapp" as "> HinvO" "HinvC".
+    iNamed "HinvO".
+    iApply ncfupd_mask_intro; first set_solver.
+    iIntros "Hmask".
+    iExists l. iFrame.
+    iIntros (l2) "Hl2".
+    iDestruct (consensus_witness with "Hl2") as "#Hlb2".
+    iMod "Hmask" as "_".
+    iMod ("HinvC" with "[Hl2 Hvs]") as "_".
+    { iDestruct (consensus_incl with "Hl2 Hvs") as %Hin.
+      do 2 iExists _. iFrame.
+      iPureIntro. split; last done.
+      unfold length_of_consensus.
+      unfold length_of_candidates in Hlenvs.
+      rewrite Forall_forall.
+      intros x Hx.
+      rewrite Forall_forall in Hin.
+      specialize (Hin _ Hx).
+      by specialize (Hlenvs _ Hin).
+    }
+    iIntros "!>" (v2 ok2 Hv2).
+    wp_pures.
+    clear Hlenl Hlenvs l vs.
+
+    (*@     if ok1 && ok2 {                                                     @*)
+    (*@         machine.Assert(v1 == v2)                                        @*)
+    (*@         // @len not supported in Goose                                  @*)
+    (*@         // machine.Assert(len(v1) == 5)                                 @*)
+    (*@     }                                                                   @*)
+    (*@                                                                         @*)
+    wp_apply (wp_and_pure (ok1 = true) (ok2 = true)).
+    { wp_pures. iPureIntro.
+      case_bool_decide as H; first by rewrite H.
+      rewrite not_true_iff_false in H. by rewrite H.
+    }
+    { iIntros (_). wp_pures. iPureIntro.
+      case_bool_decide as H; first by rewrite H.
+      rewrite not_true_iff_false in H. by rewrite H.
+    }
+    wp_if_destruct; last by iApply "HΦ".
+    destruct Heqb as [Hok1 Hok2]. subst ok1 ok2.
+    iDestruct (consensus_lb_prefix with "Hlb1 Hlb2") as %Hprefix.
+    rewrite -(prefix_lookup_same_index Hprefix Hv1 Hv2).
+    wp_apply wp_Assert; first by rewrite bool_decide_eq_true.
+    wp_pures.
+    by iApply "HΦ".
+  Qed.
+
+End prog.
+(* TODO: move to mpaxos_examples.v once stable *)
